latest updates; syntax changes; added test

PrincipiaMetaphysicaAutomationPart1/TheoryOfAbstractObjectsV1.thy
@@ -1,125 +1,214 @@
-(*<*) 
+(**) 
 theory TheoryOfAbstractObjectsV1
 imports Main
 
 begin
-(*>*)
+(**)
 
 section {* Introduction *}
-text {* This work is related to \cite{J23}, which is significantly extends ... *}
+ text {* 
+ We present a formalisation and partial automation of an initial part of the (third authors)
+ Principia Metaphysica \cite{zalta:_princ_metap} in Isabelle/HOL \cite{Isabelle}.  
+
+ The Principia Metaphysica, which is based on and extends the Theory of Abstract 
+ Objects \cite{zalta83:_abstr_objec}, 
+ employs a modal relational type theory as logical foundation. Arguments
+ defending this choice against a modal functional type theory 
+ have been presented before \cite{zalta11:_relat_versus_funct_found_logic}.
+ In a nutshell, the situation is this: functional type theory comes with strong 
+ comprehension principles, which, in the context of the Theory of Abstract Objects, 
+ have paradoxical implications. When starting off with a relational foundation, however, 
+ weaker comprehension principles are provided, and these obstacles can be avoided.
+
+ Isabelle/HOL is a proof assistant based on a functional type theory, 
+ more precisely, Church's theory of types \cite{Church40}. Recently, it has been shown 
+ that Church's type theory can be elegantly utilized as a meta-logic to encode and 
+ automate various quantified non-classical logics, including modal functional type 
+ theory \cite{J23,C40}. This work has subsequently been employed in a case study in
+ computational metaphysics, in which different variants of Kurt Gödel's ontological 
+ argument \cite{ECAI} were verified (respectively, falsified). 
+ 
+
+ The motivating research questions for the work presented below include:
+ \begin{itemize} 
+ \item Can functional type theory, despite the problems as pointed by Zalta and Oppenheimer, 
+  be utilized to encode the Theory of Abstract Objects when following the embeddings approach?
+ \item How elegant and user-friendly is the resulting formalization? In other
+  words, to what extend can Isabelle's  user interface be facilitated to hide 
+  unpleasant technicalities of the (extended) embedding from the user?
+ \item How far can automation be pushed in the approach? How much user interaction can
+  be avoided in the formalization of the (first part) of the Principia Metaphysica? 
+ \item Can the consistency of the theory be validated with the available automated 
+  reasoning tools?
+ \item Can the reasoners eventually even contribute some new knowledge? 
+ \ldots
+ \end{itemize}
+ *}
+
+ text {* The encoding of modal functional type theory in functional type theory as explored in 
+ previous work \cite{J23,C40} is simple: modal logic formulas are identified with certain functional 
+ type theory formulas of predicate type @{text "io"}. Possible worlds are explicitly represented by 
+ terms of type  @{text "i"}. A modal logic @{text "\<phi>"} formula holds for a world @{text "w"} if and 
+ only if the application @{text "\<phi> w"} evaluates to true. The definition of the propositional modal logic 
+ connectives is then straightforward and it simply realizes the standard translation as a set of equations 
+ in functional type theory. The approach has been successfully extended for quantifiers. A crucial 
+ aspect thereby is that in simple type theory quantifiers can be treated
+ as ordinary logical connectives. No extra binding mechanism is needed since the already existing 
+ lambda binding mechanism can be elegantly utilized. 
+  
+ The challenge in this work is to appropriately 'restrict' this embedding for modal relational type theory.
+  \begin{figure}[t]
+ \includegraphics[height=5.5cm]{ModalRelationalTypeTheory.png}\includegraphics[height=4.5cm]{ModalRelationalTypeTheory2.png}
+ \caption{Grammar of Modal Relational Type Theory. \label{mmrt}
+ Note that two kinds of (complex) formulas are introduced: ones that may have encoding subformulas and ones that don’t.
+ The latter are designated as propositional formulas, the former ones simply as formulas. }
+ \end{figure}
+
+
+ To achieve this  we provide means to explicitly represents and maintain information and constraints on the 
+ syntactical structure of modal relational type theory, in particular, we provide means to distinguish 
+ between propositional formulas, formulas, terms and erreneous (disallowed) formations. 
+ This clearly creates some technical overhead. However, we exploit facilities in Isabelle/HOL's user 
+ interface, and other means, to hide most of these technicalities from the user in applications. 
+   
+ *}
+
 
 section {* Preliminaries *}
-typedecl i
--- "the type possible worlds; the formalism explicitly encodes Kripke style semantics"
-type_synonym io = "(i \<Rightarrow> bool)" 
--- "formulas are essentially of this type"
--- "predicates on worlds"
-typedecl e
--- "the raw type of entities/objects (abstract or ordinary)"
-datatype 'a opt = Error 'a | Term 'a | Form 'a | PropForm 'a
+ text {* 
+ We start out with some type declarations and type abbreviations. 
+ Our formalism explicitly encodes Kripke style semantics. Hence, we introduce a 
+ distinguished type @{text "i"} to represent the set of possible worlds. 
+ Consequently, terms of this type denote possible worlds. 
+ Moreover, modal logic formulas are associated in our approach with
+ predicates (resp. sets) on possible worlds. Hence, modal logic formulas have
+ type @{text "(i \<Rightarrow> bool)"}. To make our representation in the remainder more concise
+ we abbreviate this type as @{text "io"}.
+ *}
 
+typedecl i
+type_synonym io = "(i \<Rightarrow> bool)" 
+
+ text {*
+ Entities in the abstract theory of types are represented in our formalism by the
+ type @{text "e"}. We call this the raw type of entities resp. objects. Later 
+ on we will introduce means to distinguish between abstract and ordinary entities.    
+ *}
+
+typedecl e
+
+ text {*
+ To explicitly model the syntactical restrictions of modal relational type theory we introduce a 
+ datatype @{text "'a opt"} based on four constructors:
+ @{text "ERR 'a"} (identifies erroneous term constructions), @{text "P 'a"} (identifies 
+ propositional formulas), @{text "F 'a"} (identifies  formulas), and @{text "T 'a"} (identifies 
+ terms, such as lambda abstractions). The embeddings approach will be suitably adapted below so that 
+ for each language expression (in the embedded modal relational type theory) the respective datatype 
+ is identified and appropriately propagated. The encapsulated expressions (the polymorphic type @{text "'a"} 
+ will be instantiated below) realize the actual modeling of the logic embedding analogous 
+ to previous work for modal functional type theory.  
+ *}
+
+datatype 'a opt = ERR 'a | P 'a | F 'a | T 'a 
+
+ text {* Some language constructs in the theory of abstract types, e.g. the actuality operator  
+ @{text "\<A>"} (for "it is actually the case that"), refer to a (fixed) given world. To model such a 
+ global world reference we introduce a
+ constant symbol (name) @{text "cw"} of world type @{text "i"}. Moreover, for technical reasons, 
+ which will be clarified below, we introduce further (dummy) constant symbols for various domains. Since
+ we assume that all domains are non-empty, introducing these constant symbols is obviously not harmful. 
+ *}
 
 consts cw :: i 
--- "the distinguished actual world"
-consts dE::"e" dIO::"io" dEIO::"e\<Rightarrow>io" dEEIO::"e\<Rightarrow>e\<Rightarrow>io" dEEEIO::"e\<Rightarrow>e\<Rightarrow>e\<Rightarrow>io" dA::'a
--- "some fixed dummy symbols; we anyway assume that the domains are non-empty"
--- "needed as dummy object in some cases below"
+consts de::"e" dio::"io" da::'a
 
-(* 'a indicates polymorphism *)
+section {* Embedding of Modal Relational Type Theory *}
 
+ text {* The language constructs of modal relational type theory are introduced step by step. 
+ *}
 
-section {* Encoding of the language *}
+ text {* The actuality operator @{text "\<A>"} when applied to a formula or propositional formula 
+ @{text "\<phi>"} evaluates @{text "\<phi>"} wrt the fixed given world @{text "cw"}. 
+ The compound expression @{text "\<A> \<phi>"} inherits its syntactical category  (@{text "Form"} or
+ @{text "PropForm"}) from @{text "\<phi>"}. If the syntactical catagory of  @{text "\<phi>"} is 
+ @{text "Error"} or @{text "Term"}, then the syntactical catagory of @{text "\<A> \<phi>"} 
+ is @{text "Error"} and a dummy entity of appropriate type is returned. This illustrates the very 
+ idea of our explicit structure and constraints and this scheme will repeated below
+ for all the other language constructs of modal relational type theory. 
+ *}
 
 abbreviation \<A>::"io opt \<Rightarrow> io opt" where "\<A> \<phi> \<equiv> case \<phi> of 
-    Form \<psi> \<Rightarrow> Form (\<lambda>w. \<psi> cw)
-  | PropForm \<psi> \<Rightarrow> PropForm (\<lambda>w. \<psi> cw)
-  | _ \<Rightarrow> Error dIO"
-text {* actuality operator; @{text "\<phi>"} is evaluated wrt the current world; Error is passed on *}
+    F \<psi> \<Rightarrow> F(\<lambda>w. \<psi> cw) | P \<psi> \<Rightarrow> P(\<lambda>w. \<psi> cw) | _ \<Rightarrow> ERR dio"
 
-abbreviation Enc::"e opt\<Rightarrow>(e\<Rightarrow>io) opt\<Rightarrow>io opt"(*<*)("<_\<circ>_>")(*>*) where "<x\<circ>P> \<equiv> case (x,P) of 
-    (Term y,Term Q) \<Rightarrow> Form (\<lambda>w.(Q y) w)   
-  | (_,_) \<Rightarrow> Error dIO"
-text {* @{text "\<kappa>\<^sub>1\<Pi>\<^sup>1"} will be written here as @{text "<\<kappa>\<^sub>1\<circ>\<Pi>\<^sup>1>"}; @{text "\<kappa>\<^sub>1\<Pi>\<^sup>1"} is a Form; Error is passed on *}
+ text {* The Principia Metaphysica distinguishes between encoding and exemplifying, ... say more ...
 
-abbreviation Exe1::"(e\<Rightarrow>io) opt\<Rightarrow>e opt\<Rightarrow>io opt"(*<*)("<_\<bullet>_>")(*>*) where "<P\<bullet>x> \<equiv> case (P,x) of 
-    (Term Q,Term y) \<Rightarrow> PropForm (\<lambda>w.(Q y) w)
-  | _ \<Rightarrow> Error dIO"
-text {* @{text "\<Pi>\<^sup>1\<kappa>\<^sub>1"}  will be written here as @{text "<\<Pi>\<^sup>2\<bullet>\<kappa>\<^sub>1>"}; @{text "\<Pi>\<^sup>1\<kappa>\<^sub>1 "} is a PropForm; Error is passed on *}
-
-abbreviation Exe2::"(e\<Rightarrow>e\<Rightarrow>io) opt\<Rightarrow>e opt\<Rightarrow>e opt\<Rightarrow>io opt"(*<*)("<_\<bullet>_,_>")(*>*) where "<P\<bullet>x1,x2> \<equiv> case (P,x1,x2) of 
-    (Term Q,Term y1,Term y2) \<Rightarrow> PropForm (\<lambda>w.(Q y1 y2) w)
-  | _ \<Rightarrow> Error dIO"
-text {* @{text "\<Pi>\<^sup>2\<kappa>\<^sub>1\<kappa>\<^sub>2"}   will be written here as @{text "<\<Pi>\<^sup>2\<bullet>\<kappa>\<^sub>1,\<kappa>\<^sub>2>"}; @{text "\<Pi>\<^sup>2\<kappa>\<^sub>1\<kappa>\<^sub>2"} is a PropForm; Error is passed on *}
-
-abbreviation Exe3::"(e\<Rightarrow>e\<Rightarrow>e\<Rightarrow>io) opt\<Rightarrow>e opt\<Rightarrow>e opt\<Rightarrow>e opt\<Rightarrow>io opt"(*<*)("<_\<bullet>_,_,_>") (*>*) where "<P\<bullet>x1,x2,x3> \<equiv> case (P,x1,x2,x3) of 
-    (Term Q,Term y1,Term y2,Term y3) \<Rightarrow> PropForm (\<lambda>w.(Q y1 y2 y3) w)
-  | _ \<Rightarrow> Error dIO"
-text {* @{text "\<Pi>\<^sup>3\<^sub>1\<kappa>\<^sub>2\<kappa>\<^sub>3"}  will be written here as @{text "<\<Pi>\<^sup>2\<bullet>\<kappa>\<^sub>1,\<kappa>\<^sub>2,\<kappa>\<^sub>3>"}; @{text "\<Pi>\<^sup>3\<^sub>1\<kappa>\<^sub>2\<kappa>\<^sub>3"} is a PropForm; Error is passed on; 
-we could, of course, introduce further operators: Exe4, Exe5, etc. *}
+ Encoding @{text "\<kappa>\<^sub>1\<Pi>\<^sup>1"} is noted here as @{text "\<kappa>\<^sub>1\<cdot>\<Pi>\<^sup>1"}. 
+ Encoding yields formulas and never propositional formulas. In the embedding encoding 
+ is identified with predicate application.
+ *}
 
 
-abbreviation z_not::"io opt\<Rightarrow>io opt"(*<*)("\<^bold>\<not>")(*>*) 
-  where "\<^bold>\<not> \<phi> \<equiv> case \<phi> of 
-    Form \<psi> \<Rightarrow> Form (\<lambda>w. \<not> \<psi> w)
-  | PropForm \<psi> \<Rightarrow> PropForm (\<lambda>w. \<not> \<psi> w)
-  | _ \<Rightarrow> Error dIO"  
-text {* negation operator; @{text "\<not>\<^sup>z \<phi>"} inherits its type from @{text "\<phi>"} if @{text "\<phi>"} is Form or PropForm; 
-Error is passed on *}
- 
-abbreviation z_implies::"io opt\<Rightarrow>io opt\<Rightarrow>io opt"(*<*)(infixr "\<^bold>\<rightarrow>" 51)(*>*) 
-  where "\<phi> \<^bold>\<rightarrow> \<psi> \<equiv> case (\<phi>,\<psi>) of 
-    (PropForm \<alpha>,PropForm \<beta>) \<Rightarrow> PropForm (\<lambda>w. \<alpha> w \<longrightarrow> \<beta> w)
-  | (Form \<alpha>,Form \<beta>) \<Rightarrow> Form (\<lambda>w. \<alpha> w \<longrightarrow> \<beta> w)
-  | _ \<Rightarrow> Error dIO"  
-text {* implication operator; @{text "\<phi> \<rightarrow>\<^sup>z \<psi>"} returns returns a PropForm if both are PropForms, Form if both are Forms,
-otherwise it returns Error *}
+abbreviation Enc::"e opt\<Rightarrow>(e\<Rightarrow>io) opt\<Rightarrow>io opt"(**)("_\<cdot>_")(**) where "x\<cdot>\<Phi> \<equiv> case (x,\<Phi>) of 
+    (T y,T Q) \<Rightarrow> F (\<lambda>w.(Q y) w) | _ \<Rightarrow> ERR dio"
 
-abbreviation z_forall::"('a\<Rightarrow>io opt)\<Rightarrow>io opt"(*<*)("\<^bold>\<forall>")(*>*) 
-  where "\<^bold>\<forall> \<Phi> \<equiv> case (\<Phi> dA) of
-    PropForm \<phi> \<Rightarrow> PropForm (\<lambda>w. \<forall>x. case (\<Phi> x) of PropForm \<psi> \<Rightarrow> \<psi> w)
-  | Form \<phi> \<Rightarrow> Form (\<lambda>w. \<forall>x. case (\<Phi> x) of Form \<psi> \<Rightarrow> \<psi> w)
-  | _ \<Rightarrow> Error dIO"
-text {* universal quantification; @{text "\<forall>(\<lambda>x.\<phi>)"} inherits its kind (Form or PropForm) from @{text "\<phi>"}; Error is passed on
-@{text "\<forall>(\<lambda>x.\<phi>)"} is mapped to @{text "(\<lambda>w.\<forall>x.\<phi>xw)"} as expected *}
+ text {* Exemplifying formulas @{text "\<Pi>\<^sup>1\<kappa>\<^sub>1"} are noted here as @{text "\<Pi>\<^sup>1\<bullet>\<kappa>\<^sub>1"}.  
+ Exemplification yields propositional formulas and never formulas. In the embedding exemplification 
+ is identified with predicate application, just as encoding.
+ *}
 
-abbreviation z_box::"io opt\<Rightarrow>io opt"(*<*)("\<^bold>\<box>")(*>*) 
-  where "\<^bold>\<box> \<phi> \<equiv> case \<phi> of 
-    Form \<psi> \<Rightarrow> Form (\<lambda>w. \<forall>v. \<psi> v)
-  | PropForm \<psi> \<Rightarrow> PropForm (\<lambda>w. \<forall>v. \<psi> v)
-  | _ \<Rightarrow> Error dIO"  
-text {* box operator; @{text "\<box> \<phi>"} inherits its type (Form or PropForm) from @{text "\<phi>"}; Error is passed on.
-Note that the @{text "\<box>"}-operator is defined here without an accessibility relation; this is ok since we assume logic S5. *} 
+abbreviation Exe1::"(e\<Rightarrow>io) opt\<Rightarrow>e opt\<Rightarrow>io opt"(**)("_\<bullet>_")(**) where "\<Phi>\<bullet>x \<equiv> case (\<Phi>,x) of 
+    (T Q,T y) \<Rightarrow> P (\<lambda>w.(Q y) w) | _ \<Rightarrow> ERR dio"
 
-abbreviation lam0::"io opt\<Rightarrow>io opt"(*<*)("\<lambda>\<^sup>0")(*>*) where "\<lambda>\<^sup>0 \<phi> \<equiv> case \<phi> of 
-    PropForm \<psi> \<Rightarrow> PropForm \<psi>
-  | _ \<Rightarrow> Error dIO"  
-text {* 0-arity lambda abstraction; @{text "\<lambda>\<^sup>0 \<phi>"} returns PropForm @{text "\<phi>"} if @{text "\<phi>"} is a PropForm, otherwise Error *}
+ text {* The Principia Metaphysica supports $n$-ary exemplification constructions. For pragmatical 
+ reasons we consider here the cases only for $n\leq 3$.
+ *}  
 
-abbreviation lam1::"(e\<Rightarrow>io opt)\<Rightarrow>(e\<Rightarrow>io) opt"(*<*)("\<lambda>\<^sup>1")(*>*) 
-  where "\<lambda>\<^sup>1 \<Phi> \<equiv> case (\<Phi> dE) of
-    PropForm \<phi> \<Rightarrow> Term (\<lambda>x. case (\<Phi> x) of PropForm \<phi> \<Rightarrow> \<phi>)
-  | _ \<Rightarrow> Error (\<lambda>x. dIO)"
-text {* 1-arity lambda abstraction; @{text "\<lambda>\<^sup>1(\<lambda>x.\<phi>)"} returns Term @{text "(\<lambda>x.\<phi>)"} if @{text "\<phi>"} is a PropForm, 
-otherwise Error *}
+abbreviation Exe2::"(e\<Rightarrow>e\<Rightarrow>io) opt\<Rightarrow>e opt\<Rightarrow>e opt\<Rightarrow>io opt"(**)("_\<bullet>_,_")(**) where "\<Phi>\<bullet>x1,x2 \<equiv> case (\<Phi>,x1,x2) of 
+    (T Q,T y1,T y2) \<Rightarrow> P(\<lambda>w.(Q y1 y2) w) | _ \<Rightarrow> ERR dio"
+abbreviation Exe3::"(e\<Rightarrow>e\<Rightarrow>e\<Rightarrow>io) opt\<Rightarrow>e opt\<Rightarrow>e opt\<Rightarrow>e opt\<Rightarrow>io opt"(**)("_\<bullet>_,_,_") (**) where "\<Phi>\<bullet>x1,x2,x3 \<equiv> case (\<Phi>,x1,x2,x3) of 
+    (T Q,T y1,T y2,T y3) \<Rightarrow> P (\<lambda>w.(Q y1 y2 y3) w) | _ \<Rightarrow> ERR dio"
 
-abbreviation lam2::"(e\<Rightarrow>e\<Rightarrow>io opt)\<Rightarrow>(e\<Rightarrow>e\<Rightarrow>io) opt"(*<*)("\<lambda>\<^sup>2")(*>*) 
-  where "\<lambda>\<^sup>2 \<Phi> \<equiv> case (\<Phi> dE dE) of
-    PropForm \<phi> \<Rightarrow> Term (\<lambda>x y. case (\<Phi> x y) of PropForm \<phi> \<Rightarrow> \<phi>)
-  | _ \<Rightarrow> Error (\<lambda>x y. dIO)"
-text {* 2-arity lambda abstraction; @{text "\<lambda>\<^sup>2(\<lambda>xy.\<phi>)"} returns Term @{text "(\<lambda>xy.\<phi>)"} if @{text "\<phi>"} is a PropForm, 
-otherwise Error *}
+ text {* Formations with negation and implication are supported for both, formulas  and propositional
+ formulas, and their embeddings are straightforward.
+ *}  
 
-abbreviation lam3::"(e\<Rightarrow>e\<Rightarrow>e\<Rightarrow>io opt)\<Rightarrow>(e\<Rightarrow>e\<Rightarrow>e\<Rightarrow>io) opt"(*<*)("\<lambda>\<^sup>3")(*>*) 
-  where "\<lambda>\<^sup>3 \<Phi> \<equiv> case (\<Phi> dE dE dE) of
-    PropForm \<phi> \<Rightarrow> Term (\<lambda>x y z. case (\<Phi> x y z) of PropForm \<phi> \<Rightarrow> \<phi>)
-  | _ \<Rightarrow> Error (\<lambda>x y z. dIO)"
-text {* 3-arity lambda abstraction; @{text "\<lambda>\<^sup>2(\<lambda>xyz.\<phi>)"} returns Term @{text "(\<lambda>xyz.\<phi>)"} if @{text "\<phi>"} is a PropForm, 
-otherwise Error; we could, of course, introduce further operators: @{text "\<lambda>\<^sup>4"}, @{text "\<lambda>\<^sup>5"}, etc. *}
+abbreviation negation::"io opt\<Rightarrow>io opt"(**)("\<^bold>\<not>")(**) where "\<^bold>\<not> \<phi> \<equiv> case \<phi> of 
+    F \<psi> \<Rightarrow> F (\<lambda>w.\<not>(\<psi> w)) | P \<psi> \<Rightarrow> P(\<lambda>w.\<not>(\<psi> w)) | _ \<Rightarrow> ERR dio"  
+abbreviation implication::"io opt\<Rightarrow>io opt\<Rightarrow>io opt"(**)(infixl "\<^bold>\<rightarrow>" 51)(**) where "\<phi> \<^bold>\<rightarrow> \<psi> \<equiv> case (\<phi>,\<psi>) of 
+    (F \<alpha>,F \<beta>) \<Rightarrow> F(\<lambda>w. \<alpha> w \<longrightarrow> \<beta> w) | (P \<alpha>,P \<beta>) \<Rightarrow> P(\<lambda>w. \<alpha> w \<longrightarrow> \<beta> w) | _ \<Rightarrow> ERR dio"  
 
-abbreviation that::"(e\<Rightarrow>io opt)\<Rightarrow>e opt"(*<*)("\<epsilon>")(*>*) 
-  where "\<epsilon> \<Phi> \<equiv> case (\<Phi> dE) of
-    PropForm \<phi> \<Rightarrow> Term (THE x. case (\<Phi> x) of PropForm \<psi> \<Rightarrow> \<psi> cw)
-  | _ \<Rightarrow> Error dE"
+ text {* Also universal quantification @{text "\<forall>(\<lambda>x.\<phi>)"} is supported for formulas  and propositional
+ formulas. Following previous work the embedding maps @{text "\<forall>(\<lambda>x.\<phi>)"} to @{text "(\<lambda>w.\<forall>x.\<phi>xw)"}. *}
+
+abbreviation universalQuantification::"('a\<Rightarrow>io opt)\<Rightarrow>io opt"(**)("\<^bold>\<forall>")(**) where "\<^bold>\<forall> \<Phi> \<equiv> case (\<Phi> da) of
+    F \<phi> \<Rightarrow> F(\<lambda>w.\<forall>x. case (\<Phi> x) of F \<psi> \<Rightarrow> \<psi> w) | P \<phi> \<Rightarrow> P(\<lambda>w.\<forall>x. case (\<Phi> x) of P \<psi> \<Rightarrow> \<psi> w) | _ \<Rightarrow> ERR dio"
+
+ text {* The modal box operator @{text "\<box>"} .... *}
+
+abbreviation box::"io opt\<Rightarrow>io opt"(**)("\<^bold>\<box>")(**) where "\<^bold>\<box>\<phi> \<equiv> case \<phi> of 
+    F \<psi> \<Rightarrow> F(\<lambda>w.\<forall>v. \<psi> v) | P \<psi> \<Rightarrow> P(\<lambda>w.\<forall>v. \<psi> v) | _ \<Rightarrow> ERR dio"  
+
+ text {* n-ary lambda abstraction @{text "\<lambda>\<^sup>0,\<lambda>\<^sup>1,\<lambda>\<^sup>2,\<lambda>\<^sup>3,..."}, for $n\geq 0$, is supported in the Principia
+ Metaphysica only for propositional formulas. ... say more about @{text "\<lambda>\<^sup>0"} ... Their embedding is 
+ straightforward: @{text "\<lambda>\<^sup>0"} is mapped to identity and {text "\<lambda>\<^sup>1,\<lambda>\<^sup>2,\<lambda>\<^sup>3,..."} are mapped to n-ary
+ lambda abstractions, that is, @{text "\<lambda>\<^sup>2(\<lambda>xy.\<phi>)"} is e.g. mapped to @{text "(\<lambda>xy.\<phi>)"}.
+ For pragmatical reasons we restrict ourselves here to the cases where $n\leq 0$. 
+ *}
+
+abbreviation lambda0::"io opt\<Rightarrow>io opt"(**)("\<lambda>\<^sup>0_")(**) where "\<lambda>\<^sup>0\<phi> \<equiv> case \<phi> of 
+    P \<psi> \<Rightarrow> P \<psi> | _ \<Rightarrow> ERR dio"  
+abbreviation lambda1::"(e\<Rightarrow>io opt)\<Rightarrow>(e\<Rightarrow>io) opt"(**)("\<lambda>\<^sup>1_")(**) where "\<lambda>\<^sup>1\<Phi> \<equiv> case (\<Phi> de) of
+    P \<phi> \<Rightarrow> T (\<lambda>x. case (\<Phi> x) of P \<phi> \<Rightarrow> \<phi>) | _ \<Rightarrow> ERR (\<lambda>x. dio)"
+abbreviation lambda2::"(e\<Rightarrow>e\<Rightarrow>io opt)\<Rightarrow>(e\<Rightarrow>e\<Rightarrow>io) opt"(**)("\<lambda>\<^sup>2_")(**) where "\<lambda>\<^sup>2\<Phi> \<equiv> case (\<Phi> de de) of
+    P \<phi> \<Rightarrow> T (\<lambda>x y. case (\<Phi> x y) of P \<phi> \<Rightarrow> \<phi>) | _ \<Rightarrow> ERR (\<lambda>x y. dio)"
+abbreviation lambda3::"(e\<Rightarrow>e\<Rightarrow>e\<Rightarrow>io opt)\<Rightarrow>(e\<Rightarrow>e\<Rightarrow>e\<Rightarrow>io) opt"(**)("\<lambda>\<^sup>3_")(**) where "\<lambda>\<^sup>3\<Phi> \<equiv> case (\<Phi> de de de) of
+    P \<phi> \<Rightarrow> T (\<lambda>x y z. case (\<Phi> x y z) of P \<phi> \<Rightarrow> \<phi>) | _ \<Rightarrow> ERR (\<lambda>x y z. dio)"
+
+ text {* That ...
+ *}
+
+abbreviation definiteDescription::"(e\<Rightarrow>io opt)\<Rightarrow>e opt"(**)("\<epsilon>")(**)  where "\<epsilon> \<Phi> \<equiv> case (\<Phi> de) of
+    P \<phi> \<Rightarrow> T (THE x. case (\<Phi> x) of P \<psi> \<Rightarrow> \<psi> cw) | _ \<Rightarrow> ERR de"
 text {* that operator; that @{text "(\<lambda>x.\<phi>)"} returns Term @{text "(THE x. \<phi> x cw)"}, that is the inbuilt THE 
 operator is used and evaluation is wrt to the current world cw; moreover, application of that 
 is allowed if @{text "(\<Phi> sRE)"} is a PropForm, otherwise Error is passed on for some someRawEntity *}
@@ -128,55 +217,50 @@ is allowed if @{text "(\<Phi> sRE)"} is a PropForm, otherwise Error is passed on
 
 section {* Further logical connectives *}
 
-abbreviation z_and::"io opt\<Rightarrow>io opt\<Rightarrow>io opt"(*<*)(infixr "\<^bold>\<and>" 53)(*>*) where "\<phi> \<^bold>\<and> \<psi> \<equiv> \<^bold>\<not>(\<phi> \<^bold>\<rightarrow> \<^bold>\<not>\<psi>)"
-abbreviation z_or::"io opt\<Rightarrow>io opt\<Rightarrow>io opt"(*<*)(infixr "\<^bold>\<or>" 52)(*>*) where "\<phi> \<^bold>\<or> \<psi> \<equiv> \<^bold>\<not>\<phi> \<^bold>\<rightarrow> \<psi>"
-abbreviation z_equiv::"io opt\<Rightarrow>io opt\<Rightarrow>io opt"(*<*)(infixr "\<^bold>\<equiv>" 52)(*>*) where "\<phi> \<^bold>\<equiv> \<psi> \<equiv> (\<phi> \<^bold>\<rightarrow> \<psi>) \<^bold>\<and> (\<psi> \<^bold>\<rightarrow> \<phi>)"
-abbreviation z_exists::"('a\<Rightarrow>io opt)\<Rightarrow>io opt"(*<*)("\<^bold>\<exists>")(*>*) where "\<^bold>\<exists> \<Phi> \<equiv> case (\<Phi> dA) of
-    PropForm \<phi> \<Rightarrow> PropForm (\<lambda>w. \<exists>x. case (\<Phi> x) of PropForm \<psi> \<Rightarrow> \<psi> w)
-  | Form \<phi> \<Rightarrow> Form (\<lambda>w. \<exists>x. case (\<Phi> x) of Form \<psi> \<Rightarrow> \<psi> w)
-  | _ \<Rightarrow> Error dIO"
-abbreviation z_dia::"io opt\<Rightarrow>io opt"(*<*)("\<^bold>\<diamond>")(*>*) where "\<^bold>\<diamond> \<phi> \<equiv> \<^bold>\<not>(\<^bold>\<box>(\<^bold>\<not> \<phi>))"
+abbreviation conjunction::"io opt\<Rightarrow>io opt\<Rightarrow>io opt"(**)(infixl "\<^bold>\<and>" 53)(**) where "\<phi>\<^bold>\<and>\<psi> \<equiv> \<^bold>\<not>(\<phi>\<^bold>\<rightarrow>\<^bold>\<not>\<psi>)"
+abbreviation disjunction::"io opt\<Rightarrow>io opt\<Rightarrow>io opt"(**)(infixl "\<^bold>\<or>" 52)(**) where "\<phi>\<^bold>\<or>\<psi> \<equiv> \<^bold>\<not>\<phi>\<^bold>\<rightarrow>\<psi>"
+abbreviation equivalence::"io opt\<Rightarrow>io opt\<Rightarrow>io opt"(**)(infixl "\<^bold>\<equiv>" 52)(**) where "\<phi>\<^bold>\<equiv>\<psi> \<equiv> (\<phi>\<^bold>\<rightarrow>\<psi>)\<^bold>\<and>(\<psi>\<^bold>\<rightarrow>\<phi>)"
+abbreviation diamond::"io opt\<Rightarrow>io opt"(**)("\<^bold>\<diamond>")(**) where "\<^bold>\<diamond>\<phi> \<equiv> \<^bold>\<not>(\<^bold>\<box>(\<^bold>\<not> \<phi>))"
+abbreviation existentialQuantification::"('a\<Rightarrow>io opt)\<Rightarrow>io opt"(**)("\<^bold>\<exists>")(**) where "\<^bold>\<exists>\<Phi> \<equiv> case (\<Phi> da) of
+    P \<phi> \<Rightarrow> P(\<lambda>w.\<exists>x. case (\<Phi> x) of P \<psi> \<Rightarrow> \<psi> w) | F \<phi> \<Rightarrow> F(\<lambda>w. \<exists>x. case (\<Phi> x) of F \<psi> \<Rightarrow> \<psi> w) | _ \<Rightarrow> ERR dio"
 
-(* abbreviation z_true::"io opt"(*<*)("\<top>\<^sup>z")(*>*) where "\<top>\<^sup>z \<equiv> todo; not entirely clear yet " *)
-(* abbreviation z_false::"io opt"(*<*)("\<bottom>\<^sup>z")(*>*) where "\<bottom>\<^sup>z \<equiv> todo; not entirely clear yet " *)
+(* abbreviation z_true::"io opt"(**)("\<top>\<^sup>z")(**) where "\<top>\<^sup>z \<equiv> todo; not entirely clear yet " *)
+(* abbreviation z_false::"io opt"(**)("\<bottom>\<^sup>z")(**) where "\<bottom>\<^sup>z \<equiv> todo; not entirely clear yet " *)
 
 
 section {* Some shortcuts for the constructors *}
 
-abbreviation mkPropForm ::  "io\<Rightarrow>io opt"(*<*)(",_,")(*>*)  where ",p, \<equiv> PropForm p" 
-abbreviation mkForm ::  "io\<Rightarrow>io opt"(*<*)(";_;")(*>*)  where ";p; \<equiv> Form p" 
-abbreviation mkTerm ::  "'a\<Rightarrow>'a opt"(*<*)("._.")(*>*)  where ".t. \<equiv> Term t" 
-abbreviation mkError ::  "'a\<Rightarrow>'a opt"(*<*)("*_*")(*>*)  where "*t* \<equiv> Term t" 
+abbreviation mkPropForm::"io\<Rightarrow>io opt" ("_\<^sup>P" 110)  where "\<phi>\<^sup>P \<equiv> P \<phi>" 
+abbreviation mkForm::"io\<Rightarrow>io opt" ("_\<^sup>F" 110)  where "\<phi>\<^sup>F \<equiv> F \<phi>" 
+abbreviation mkTerm::"'a\<Rightarrow>'a opt" ("_\<^sup>T" 110)  where "\<phi>\<^sup>T \<equiv> T \<phi>" 
 
 
+ text {* Three Valued Meta-Logic *}
 
-
-text {* Three Valued Meta-Logic *}
-
-datatype mf = tt | ff | error
+datatype mf = tt ("\<top>") | ff ("\<bottom>") | err ("*")
 
 (*
-abbreviation meta_not::"mf \<Rightarrow> mf" (*<*)("\<not>\<^sup>m")(*>*) 
+abbreviation meta_not::"mf \<Rightarrow> mf" (**)("\<not>\<^sup>m")(**) 
   where "\<not>\<^sup>m \<phi>  \<equiv> case \<phi> of 
     error \<Rightarrow> error | tt \<Rightarrow> ff | ff \<Rightarrow> tt"  
 text {* Not operator *}
 
-abbreviation meta_implies::"mf \<Rightarrow> mf \<Rightarrow>mf" (*<*)(infixr "\<longrightarrow>\<^sup>m" 51)(*>*) 
+abbreviation meta_implies::"mf \<Rightarrow> mf \<Rightarrow>mf" (**)(infixr "\<longrightarrow>\<^sup>m" 51)(**) 
   where "\<phi> \<longrightarrow>\<^sup>m \<psi> \<equiv> case (\<phi>,\<psi>) of 
     (error,_) \<Rightarrow> error | (_,error) \<Rightarrow> error | (tt,ff) \<Rightarrow> ff | _ \<Rightarrow> tt"  
 text {* Implies operator *}
 
-abbreviation meta_or::"mf \<Rightarrow> mf \<Rightarrow>mf" (*<*)(infixr "\<or>\<^sup>m" 51)(*>*) 
+abbreviation meta_or::"mf \<Rightarrow> mf \<Rightarrow>mf" (**)(infixr "\<or>\<^sup>m" 51)(**) 
   where "\<phi> \<or>\<^sup>m \<psi> \<equiv> case (\<phi>,\<psi>) of 
     (error,_) \<Rightarrow> error | (_,error) \<Rightarrow> error | (ff,ff) \<Rightarrow> ff | _ \<Rightarrow> tt"  
 text {* Or operator *}
 
-abbreviation meta_and::"mf \<Rightarrow> mf \<Rightarrow>mf" (*<*)(infixr "\<and>\<^sup>m" 51)(*>*) 
+abbreviation meta_and::"mf \<Rightarrow> mf \<Rightarrow>mf" (**)(infixr "\<and>\<^sup>m" 51)(**) 
   where "\<phi> \<and>\<^sup>m \<psi> \<equiv> case (\<phi>,\<psi>) of 
     (error,_) \<Rightarrow> error | (_,error) \<Rightarrow> error | (tt,tt) \<Rightarrow> tt | _ \<Rightarrow> ff"  
 text {* And operator *}
 
-abbreviation meta_equiv::"mf \<Rightarrow> mf \<Rightarrow>mf" (*<*)(infixr "\<longleftrightarrow>\<^sup>m" 51)(*>*) 
+abbreviation meta_equiv::"mf \<Rightarrow> mf \<Rightarrow>mf" (**)(infixr "\<longleftrightarrow>\<^sup>m" 51)(**) 
   where "\<phi> \<longleftrightarrow>\<^sup>m \<psi> \<equiv> case (\<phi>,\<psi>) of 
     (error,_) \<Rightarrow> error | (_,error) \<Rightarrow> error | (tt,tt) \<Rightarrow> tt | (ff,ff) \<Rightarrow> tt | _ \<Rightarrow> ff"  
 text {* Equivalence operator *}
@@ -184,23 +268,16 @@ text {* Equivalence operator *}
 *)
 
 
-(*<*) no_syntax "_list" :: "args\<Rightarrow>e list" ("[(_)]") (*>*) 
-abbreviation valid :: "io opt\<Rightarrow>mf" (*<*)("[_]")(*>*) where "[\<phi>] \<equiv> case \<phi> of 
-    PropForm \<psi> \<Rightarrow> if \<forall>w.(\<psi> w) \<longleftrightarrow> True then tt else ff
-  | Form \<psi> \<Rightarrow> if \<forall>w.(\<psi> w) \<longleftrightarrow> True then tt else ff
-  | _ \<Rightarrow> error"
-abbreviation satisfiable :: "io opt\<Rightarrow>mf" (*<*)("[_]\<^sup>s\<^sup>a\<^sup>t")(*>*) where "[\<phi>]\<^sup>s\<^sup>a\<^sup>t \<equiv> case \<phi> of 
-    PropForm \<psi> \<Rightarrow> if \<exists>w.(\<psi> w) \<longleftrightarrow> True then tt else ff
-  | Form \<psi> \<Rightarrow> if \<exists>w.(\<psi> w) \<longleftrightarrow> True then tt else ff
-  | _ \<Rightarrow> error"
-abbreviation countersatisfiable :: "io opt\<Rightarrow>mf" (*<*)("[_]\<^sup>c\<^sup>s\<^sup>a\<^sup>t")(*>*) where "[\<phi>]\<^sup>c\<^sup>s\<^sup>a\<^sup>t \<equiv>  case \<phi> of 
-    PropForm \<psi> \<Rightarrow> if \<exists>w.\<not>(\<psi> w) \<longleftrightarrow> True then tt else ff
-  | Form \<psi> \<Rightarrow> if \<exists>w.\<not>(\<psi> w) \<longleftrightarrow> True then tt else ff
-  | _ \<Rightarrow> error"
-abbreviation invalid :: "io opt\<Rightarrow>mf" (*<*)("[_]\<^sup>i\<^sup>n\<^sup>v")(*>*) where "[\<phi>]\<^sup>i\<^sup>n\<^sup>v \<equiv> case \<phi> of 
-    PropForm \<psi> \<Rightarrow> if \<forall>w.\<not>(\<psi> w) \<longleftrightarrow> True then tt else ff
-  | Form \<psi> \<Rightarrow> if \<forall>w.\<not>(\<psi> w) \<longleftrightarrow> True then tt else ff
-  | _ \<Rightarrow> error"
+
+(**) no_syntax "_list" :: "args\<Rightarrow>e list" ("[(_)]") (**) 
+abbreviation valid :: "io opt\<Rightarrow>mf" (**)("[_]")(**) where "[\<phi>] \<equiv> case \<phi> of 
+    P \<psi> \<Rightarrow> if \<forall>w.(\<psi> w) \<longleftrightarrow> True then \<top> else \<bottom> | F \<psi> \<Rightarrow> if \<forall>w.(\<psi> w) \<longleftrightarrow> True then \<top> else \<bottom> | _ \<Rightarrow> *"
+abbreviation satisfiable :: "io opt\<Rightarrow>mf" (**)("[_]\<^sup>s\<^sup>a\<^sup>t")(**) where "[\<phi>]\<^sup>s\<^sup>a\<^sup>t \<equiv> case \<phi> of 
+    P \<psi> \<Rightarrow> if \<exists>w.(\<psi> w) \<longleftrightarrow> True then \<top> else \<bottom> | F \<psi> \<Rightarrow> if \<exists>w.(\<psi> w) \<longleftrightarrow> True then \<top> else \<bottom> | _ \<Rightarrow> *"
+abbreviation countersatisfiable :: "io opt\<Rightarrow>mf" (**)("[_]\<^sup>c\<^sup>s\<^sup>a\<^sup>t")(**) where "[\<phi>]\<^sup>c\<^sup>s\<^sup>a\<^sup>t \<equiv>  case \<phi> of 
+    P \<psi> \<Rightarrow> if \<exists>w.\<not>(\<psi> w) \<longleftrightarrow> True then \<top> else \<bottom> | F \<psi> \<Rightarrow> if \<exists>w.\<not>(\<psi> w) \<longleftrightarrow> True then \<top> else \<bottom> | _ \<Rightarrow> *"
+abbreviation invalid :: "io opt\<Rightarrow>mf" (**)("[_]\<^sup>i\<^sup>n\<^sup>v")(**) where "[\<phi>]\<^sup>i\<^sup>n\<^sup>v \<equiv> case \<phi> of 
+    P \<psi> \<Rightarrow> if \<forall>w.\<not>(\<psi> w) \<longleftrightarrow> True then \<top> else \<bottom> | F \<psi> \<Rightarrow> if \<forall>w.\<not>(\<psi> w) \<longleftrightarrow> True then \<top> else \<bottom> | _ \<Rightarrow> *"
 
 
 section {* Some Basic Tests *}
@@ -209,111 +286,108 @@ section {* Some Basic Tests *}
 subsection {* Verifying Modal Logic Principles *}
 
 text {* Necessitation holds *}
-lemma necessitation_PropForm: "[,\<phi>,] = tt \<longrightarrow> [\<^bold>\<box> ,\<phi>,] = tt" apply simp done
-lemma necessitation_Form:     "[;\<phi>;] = tt \<longrightarrow> [\<^bold>\<box> ;\<phi>;] = tt" apply simp done
+lemma necessitation_PropForm: "[\<phi>\<^sup>P] = \<top> \<longrightarrow> [\<^bold>\<box>(\<phi>\<^sup>P)] = \<top>" apply simp done
+lemma necessitation_Form:     "[\<phi>\<^sup>F] = \<top> \<longrightarrow> [\<^bold>\<box>(\<phi>\<^sup>F)] = \<top>" apply simp done
 
 text {* Modal Collapse does not hold *}
-lemma modalCollapse_PropForm: "[,\<phi>, \<^bold>\<rightarrow> \<^bold>\<box> ,\<phi>,] = tt" apply simp nitpick oops
-lemma modalCollapse_Form:     "[;\<phi>; \<^bold>\<rightarrow> \<^bold>\<box> ;\<phi>;] = tt" apply simp nitpick oops
+lemma modalCollapse_PropForm: "[\<phi>\<^sup>P \<^bold>\<rightarrow> \<^bold>\<box>(\<phi>\<^sup>P)] = \<top>" apply simp nitpick oops
+lemma modalCollapse_Form:     "[\<phi>\<^sup>F \<^bold>\<rightarrow> \<^bold>\<box>(\<phi>\<^sup>F)] = \<top>" apply simp nitpick oops
 
 
 subsection {* S5 Principles *}
 
-lemma axiom_T_PF: "[(\<^bold>\<box> ,\<phi>,) \<^bold>\<rightarrow> ,\<phi>,] = tt" apply simp done
-lemma axiom_T_F:  "[(\<^bold>\<box> ;\<phi>;) \<^bold>\<rightarrow> ;\<phi>;] = tt" apply simp done
+lemma axiom_T_P: "[\<^bold>\<box>(\<phi>\<^sup>P) \<^bold>\<rightarrow> (\<phi>\<^sup>P)] = \<top>" apply simp done
+lemma axiom_T_F: "[\<^bold>\<box>(\<phi>\<^sup>F) \<^bold>\<rightarrow> (\<phi>\<^sup>F)] = \<top>" apply simp done
 
-lemma axiom_B_PF: "[,\<phi>, \<^bold>\<rightarrow> (\<^bold>\<box> (\<^bold>\<diamond> ,\<phi>,))] = tt" apply simp done
-lemma axiom_B_F:  "[;\<phi>; \<^bold>\<rightarrow> (\<^bold>\<box> (\<^bold>\<diamond> ;\<phi>;))] = tt" apply simp done
+lemma axiom_B_P: "[\<phi>\<^sup>P \<^bold>\<rightarrow> \<^bold>\<box>(\<^bold>\<diamond>(\<phi>\<^sup>P))] = \<top>" apply simp done
+lemma axiom_B_F: "[\<phi>\<^sup>F \<^bold>\<rightarrow> \<^bold>\<box>(\<^bold>\<diamond>(\<phi>\<^sup>F))] = \<top>" apply simp done
 
-lemma axiom_D_PF: "[\<^bold>\<box> ,\<phi>, \<^bold>\<rightarrow> \<^bold>\<box> (\<^bold>\<box> ,\<phi>,)] = tt" apply simp done
-lemma axiom_D_F:  "[\<^bold>\<box> ;\<phi>; \<^bold>\<rightarrow> \<^bold>\<box> (\<^bold>\<box> ;\<phi>;)] = tt" apply simp done
+lemma axiom_4_P: "[\<^bold>\<box>(\<phi>\<^sup>P) \<^bold>\<rightarrow> \<^bold>\<diamond>(\<phi>\<^sup>P)] = \<top>" apply simp by auto
+lemma axiom_4_F: "[\<^bold>\<box>(\<phi>\<^sup>F) \<^bold>\<rightarrow> \<^bold>\<diamond>(\<phi>\<^sup>F)] = \<top>" apply simp by auto
 
-lemma axiom_4_PF: "[\<^bold>\<box> ,\<phi>, \<^bold>\<rightarrow> \<^bold>\<diamond> ,\<phi>,] = tt" apply simp by auto
-lemma axiom_4_F:  "[\<^bold>\<box> ;\<phi>; \<^bold>\<rightarrow> \<^bold>\<diamond> ;\<phi>;] = tt" apply simp by auto
+lemma axiom_D_P: "[\<^bold>\<box>(\<phi>\<^sup>P) \<^bold>\<rightarrow> \<^bold>\<box>(\<^bold>\<box>(\<phi>\<^sup>P))] = \<top>" apply simp done
+lemma axiom_D_F: "[\<^bold>\<box>(\<phi>\<^sup>F) \<^bold>\<rightarrow> \<^bold>\<box>(\<^bold>\<box>(\<phi>\<^sup>F))] = \<top>" apply simp done
 
-lemma axiom_5_PF: "[\<^bold>\<diamond> ,\<phi>, \<^bold>\<rightarrow> \<^bold>\<box> (\<^bold>\<diamond> ,\<phi>,)] = tt" apply simp done
-lemma axiom_5_F:  "[\<^bold>\<diamond> ;\<phi>; \<^bold>\<rightarrow> \<^bold>\<box> (\<^bold>\<diamond> ;\<phi>;)] = tt" apply simp done
+lemma axiom_5_P: "[\<^bold>\<diamond>(\<phi>\<^sup>P) \<^bold>\<rightarrow> \<^bold>\<box>(\<^bold>\<diamond>(\<phi>\<^sup>P))] = \<top>" apply simp done
+lemma axiom_5_F: "[\<^bold>\<diamond>(\<phi>\<^sup>F) \<^bold>\<rightarrow> \<^bold>\<box>(\<^bold>\<diamond>(\<phi>\<^sup>F))] = \<top>" apply simp done
 
+lemma test_A_P: "[\<^bold>\<box>(\<^bold>\<diamond>(\<phi>\<^sup>P)) \<^bold>\<rightarrow> \<^bold>\<diamond>(\<phi>\<^sup>P)] = \<top>" apply simp done
+lemma test_A_F: "[\<^bold>\<box>(\<^bold>\<diamond>(\<phi>\<^sup>F)) \<^bold>\<rightarrow> \<^bold>\<diamond>(\<phi>\<^sup>F)] = \<top>" apply simp done
 
-lemma test_A_PF: "[\<^bold>\<box> (\<^bold>\<diamond> ,\<phi>,) \<^bold>\<rightarrow> \<^bold>\<diamond> ,\<phi>,] = tt" apply simp done
-lemma test_A_F:  "[\<^bold>\<box> (\<^bold>\<diamond> ;\<phi>;) \<^bold>\<rightarrow> \<^bold>\<diamond> ;\<phi>;] = tt" apply simp done
+lemma test_B_P: "[\<^bold>\<diamond>(\<^bold>\<box>(\<phi>\<^sup>P)) \<^bold>\<rightarrow> \<^bold>\<diamond>(\<phi>\<^sup>P)] = \<top>" apply simp by auto
+lemma test_B_F: "[\<^bold>\<diamond>(\<^bold>\<box>(\<phi>\<^sup>F)) \<^bold>\<rightarrow> \<^bold>\<diamond>(\<phi>\<^sup>F)] = \<top>" apply simp by auto
 
-lemma test_B_PF: "[\<^bold>\<diamond> (\<^bold>\<box> ,\<phi>,) \<^bold>\<rightarrow> \<^bold>\<diamond> ,\<phi>,] = tt" apply simp by auto
-lemma test_B_F:  "[\<^bold>\<diamond> (\<^bold>\<box> ;\<phi>;) \<^bold>\<rightarrow> \<^bold>\<diamond> ;\<phi>;] = tt" apply simp by auto
+lemma test_C_P: "[\<^bold>\<box>(\<^bold>\<diamond>(\<phi>\<^sup>P)) \<^bold>\<rightarrow> \<^bold>\<box>(\<phi>\<^sup>P)] = \<top>" apply simp nitpick oops
+lemma test_C_F: "[\<^bold>\<box>(\<^bold>\<diamond>(\<phi>\<^sup>F)) \<^bold>\<rightarrow> \<^bold>\<box>(\<phi>\<^sup>F)] = \<top>" apply simp nitpick oops
 
-lemma test_C_PF: "[\<^bold>\<box> (\<^bold>\<diamond> ,\<phi>,) \<^bold>\<rightarrow> \<^bold>\<box> ,\<phi>,] = tt" apply simp nitpick oops
-lemma test_C_F:  "[\<^bold>\<box> (\<^bold>\<diamond> ;\<phi>;) \<^bold>\<rightarrow> \<^bold>\<box> ;\<phi>;] = tt" apply simp nitpick oops
-
-lemma test_D_PF: "[\<^bold>\<diamond> (\<^bold>\<box> ,\<phi>,) \<^bold>\<rightarrow> \<^bold>\<box> ,\<phi>,] = tt" apply simp done
-lemma test_D_F:  "[\<^bold>\<diamond> (\<^bold>\<box> ;\<phi>;) \<^bold>\<rightarrow> \<^bold>\<box> ;\<phi>;] = tt" apply simp done
+lemma test_D_P: "[\<^bold>\<diamond>(\<^bold>\<box>(\<phi>\<^sup>P)) \<^bold>\<rightarrow> \<^bold>\<box>(\<phi>\<^sup>P)] = \<top>" apply simp done
+lemma test_D_F: "[\<^bold>\<diamond>(\<^bold>\<box>(\<phi>\<^sup>F)) \<^bold>\<rightarrow> \<^bold>\<box>(\<phi>\<^sup>F)] = \<top>" apply simp done
 
 
 subsection {* Validity, Satisfiabilty, Countersatisfiability and Invalidity *}
-lemma  "[,\<phi>,] = tt \<longleftrightarrow> [,\<phi>,]\<^sup>c\<^sup>s\<^sup>a\<^sup>t = ff" apply simp done
-lemma  "[,\<phi>,]\<^sup>s\<^sup>a\<^sup>t = tt \<longleftrightarrow> [,\<phi>,]\<^sup>i\<^sup>n\<^sup>v = ff" apply simp done
-lemma  "[;\<phi>;] = tt \<longleftrightarrow> [;\<phi>;]\<^sup>c\<^sup>s\<^sup>a\<^sup>t = ff" apply simp done
-lemma  "[;\<phi>;]\<^sup>s\<^sup>a\<^sup>t = tt \<longleftrightarrow> [;\<phi>;]\<^sup>i\<^sup>n\<^sup>v = ff" apply simp done
+lemma  "[\<phi>\<^sup>P] = \<top> \<longleftrightarrow> [\<phi>\<^sup>P]\<^sup>c\<^sup>s\<^sup>a\<^sup>t = \<bottom>" apply simp done
+lemma  "[\<phi>\<^sup>P]\<^sup>s\<^sup>a\<^sup>t = \<top> \<longleftrightarrow> [\<phi>\<^sup>P]\<^sup>i\<^sup>n\<^sup>v = \<bottom>" apply simp done
+lemma  "[\<phi>\<^sup>F] = \<top> \<longleftrightarrow> [\<phi>\<^sup>F]\<^sup>c\<^sup>s\<^sup>a\<^sup>t = \<bottom>" apply simp done
+lemma  "[\<phi>\<^sup>F]\<^sup>s\<^sup>a\<^sup>t = \<top> \<longleftrightarrow> [\<phi>\<^sup>F]\<^sup>i\<^sup>n\<^sup>v = \<bottom>" apply simp done
 
-text {* For Terms and Error we have *}
-lemma  "[.\<phi>.] = error" apply simp done
-lemma  "[.\<phi>.]\<^sup>s\<^sup>a\<^sup>t = error" apply simp done
-lemma  "[.\<phi>.]\<^sup>c\<^sup>s\<^sup>a\<^sup>t = error" apply simp done
-lemma  "[.\<phi>.]\<^sup>i\<^sup>n\<^sup>v = error" apply simp done
-lemma  "[*\<phi>*] = error" apply simp done
-lemma  "[*\<phi>*]\<^sup>s\<^sup>a\<^sup>t = error" apply simp done
-lemma  "[*\<phi>*]\<^sup>c\<^sup>s\<^sup>a\<^sup>t = error" apply simp done
-lemma  "[*\<phi>*]\<^sup>i\<^sup>n\<^sup>v = error" apply simp done
+text {* For Terms we have *}
+lemma  "[\<phi>\<^sup>T] = *" apply simp done
+lemma  "[\<phi>\<^sup>T]\<^sup>s\<^sup>a\<^sup>t = *" apply simp done
+lemma  "[\<phi>\<^sup>T]\<^sup>c\<^sup>s\<^sup>a\<^sup>t = *" apply simp done
+lemma  "[\<phi>\<^sup>T]\<^sup>i\<^sup>n\<^sup>v = *" apply simp done
+
+
 
 subsection {* Example signature; entities and relations *}
 
-consts a_0 :: "e" abbreviation a  where "a \<equiv> .a_0."
-consts b_0 :: "e" abbreviation b  where "b \<equiv> .b_0."
-consts c_0 :: "e" abbreviation c  where "c \<equiv> .c_0."
+consts a_0 :: "e" abbreviation a  where "a \<equiv> (a_0\<^sup>T)"
+consts b_0 :: "e" abbreviation b  where "b \<equiv> (b_0\<^sup>T)"
+consts c_0 :: "e" abbreviation c  where "c \<equiv> (c_0\<^sup>T)"
 
-consts R_0 :: "io"  abbreviation R0  where "R0 \<equiv> .R_0."
-consts R_1 :: "e\<Rightarrow>io" abbreviation R1  where "R1 \<equiv> .R_1."
-consts R_2 :: "e\<Rightarrow>e\<Rightarrow>io" abbreviation R2  where "R2 \<equiv> .R_2."
-consts R_3 :: "e\<Rightarrow>e\<Rightarrow>e\<Rightarrow>io"  abbreviation R3  where "R3 \<equiv> .R_3."
+consts R_0 :: "io"  abbreviation R0  where "R0 \<equiv> (R_0\<^sup>T)"
+consts R_1 :: "e\<Rightarrow>io" abbreviation R1  where "R1 \<equiv> (R_1\<^sup>T)"
+consts R_2 :: "e\<Rightarrow>e\<Rightarrow>io" abbreviation R2  where "R2 \<equiv> (R_2\<^sup>T)"
+consts R_3 :: "e\<Rightarrow>e\<Rightarrow>e\<Rightarrow>io"  abbreviation R3  where "R3 \<equiv> (R_3\<^sup>T)"
 
 
 text {* Testing term and formula constructions *}
 
-lemma "[<R1\<bullet>a>] = tt" apply simp nitpick oops
-lemma "<R1\<bullet>a> = X" apply simp oops
+lemma "[R1\<bullet>a] = \<top>" apply simp nitpick oops
+lemma "(R1\<bullet>a) = X" apply simp oops
 
-lemma "[<a\<circ>R1>] = tt" nitpick oops
-lemma "<a\<circ>R1> = X" apply simp oops
+lemma "[a\<cdot>R1] = \<top>" nitpick oops
+lemma "(a\<cdot>R1) = X" apply simp oops
 
-lemma "[<\<lambda>\<^sup>1(\<lambda>x. <R1\<bullet>.x.> \<^bold>\<rightarrow> <R1\<bullet>.x.>)\<bullet>a>] = tt" apply simp done
-lemma "<\<lambda>\<^sup>1(\<lambda>x. <R1\<bullet>.x.> \<^bold>\<rightarrow> <R1\<bullet>.x.>)\<bullet>a> = X" apply simp oops
+lemma "[(\<lambda>\<^sup>1(\<lambda>x. (R1\<bullet>(x\<^sup>T)) \<^bold>\<rightarrow> (R1\<bullet>(x\<^sup>T))))\<bullet>a] = \<top>" apply simp done
+lemma "((\<lambda>\<^sup>1(\<lambda>x. (R1\<bullet>(x\<^sup>T)) \<^bold>\<rightarrow> (R1\<bullet>(x\<^sup>T))))\<bullet>a) = X" apply simp oops
 
-lemma "\<lambda>\<^sup>1(\<lambda>x. <R1\<bullet>.x.> \<^bold>\<rightarrow> <.x.\<circ>R1>) = X" apply simp oops
+lemma "(\<lambda>\<^sup>1(\<lambda>x. (R1\<bullet>(x\<^sup>T)) \<^bold>\<rightarrow> ((x\<^sup>T)\<cdot>R1))) = X" apply simp oops
 
-lemma "[<\<lambda>\<^sup>1(\<lambda>x. <R1\<bullet>.x.> \<^bold>\<rightarrow> <.x.\<circ>R1>)\<bullet>a>] = error" apply simp done
-lemma "[<\<lambda>\<^sup>1(\<lambda>x. <R1\<bullet>.x.> \<^bold>\<rightarrow> <.x.\<circ>R1>)\<bullet>a>] = X" apply simp oops
-lemma "<\<lambda>\<^sup>1(\<lambda>x. <R1\<bullet>.x.> \<^bold>\<rightarrow> <.x.\<circ>R1>)\<bullet>a> = X" apply simp oops
+lemma "[(\<lambda>\<^sup>1(\<lambda>x. (R1\<bullet>(x\<^sup>T)) \<^bold>\<rightarrow> (x\<^sup>T\<cdot>R1)))\<bullet>a] = *" apply simp done
+lemma "[(\<lambda>\<^sup>1(\<lambda>x. (R1\<bullet>(x\<^sup>T)) \<^bold>\<rightarrow> (x\<^sup>T\<cdot>R1)))\<bullet>a] = X" apply simp oops
+lemma "((\<lambda>\<^sup>1(\<lambda>x. (R1\<bullet>(x\<^sup>T)) \<^bold>\<rightarrow> (x\<^sup>T\<cdot>R1)))\<bullet>a) = X" apply simp oops
 
-lemma "[\<^bold>\<forall>(\<lambda>x. <R1\<bullet>.x.> \<^bold>\<rightarrow> <R1\<bullet>.x.>)] = tt" apply simp done
-lemma "[\<^bold>\<forall>(\<lambda>R. \<^bold>\<forall>(\<lambda>x. <.R.\<bullet>.x.> \<^bold>\<rightarrow> <.R.\<bullet>.x.>))] = tt" apply simp done
-lemma "\<^bold>\<forall>(\<lambda>x. <R1\<bullet>.x.> \<^bold>\<rightarrow> <R1\<bullet>.x.>) = X" apply simp oops
+lemma "[\<^bold>\<forall>(\<lambda>x. (R1\<bullet>(x\<^sup>T)) \<^bold>\<rightarrow> (R1\<bullet>(x\<^sup>T)))] = \<top>" apply simp done
+lemma "[\<^bold>\<forall>(\<lambda>R. \<^bold>\<forall>(\<lambda>x. (R1\<bullet>(x\<^sup>T)) \<^bold>\<rightarrow> (R1\<bullet>(x\<^sup>T))))] = \<top>" apply simp done
+lemma "\<^bold>\<forall>(\<lambda>x. (R1\<bullet>(x\<^sup>T)) \<^bold>\<rightarrow> (R1\<bullet>(x\<^sup>T))) = X" apply simp oops
 
-lemma "[\<^bold>\<forall>(\<lambda>x. <.x.\<circ>R1> \<^bold>\<rightarrow> <.x.\<circ>R1>)] = tt" apply simp done
-lemma "\<^bold>\<forall>(\<lambda>x. <.x.\<circ>R1> \<^bold>\<rightarrow> <.x.\<circ>R1>) = X" apply simp oops
+lemma "[\<^bold>\<forall>(\<lambda>x. (x\<^sup>T\<cdot>R1) \<^bold>\<rightarrow> (x\<^sup>T\<cdot>R1))] = \<top>" apply simp done
+lemma "\<^bold>\<forall>(\<lambda>x. (x\<^sup>T\<cdot>R1) \<^bold>\<rightarrow> (x\<^sup>T\<cdot>R1)) = X" apply simp oops
 
-lemma "[\<^bold>\<forall>(\<lambda>x. <R1\<bullet>.x.> \<^bold>\<rightarrow> <.x.\<circ>R1>)] = error" apply simp done
-lemma "[\<^bold>\<forall>(\<lambda>x. <R1\<bullet>.x.> \<^bold>\<rightarrow> <.x.\<circ>R1>)] = X" apply simp oops
-lemma "\<^bold>\<forall>(\<lambda>x. <R1\<bullet>.x.> \<^bold>\<rightarrow> <.x.\<circ>R1>) = X" apply simp oops
-lemma "[\<^bold>\<forall>(\<lambda>R. <.R.\<bullet>.x.> \<^bold>\<rightarrow> <.x.\<circ>.R.>)] = error" apply simp done
-lemma "\<^bold>\<forall>(\<lambda>R. <.R.\<bullet>.x.> \<^bold>\<rightarrow> <.x.\<circ>.R.>) = X" apply simp oops
+lemma "[\<^bold>\<forall>(\<lambda>x. (R1\<bullet>(x\<^sup>T)) \<^bold>\<rightarrow> (x\<^sup>T\<cdot>R1))] = *" apply simp done
+lemma "[\<^bold>\<forall>(\<lambda>x. (R1\<bullet>(x\<^sup>T)) \<^bold>\<rightarrow> (x\<^sup>T\<cdot>R1))] = X" apply simp oops
+lemma "\<^bold>\<forall>(\<lambda>x. (R1\<bullet>(x\<^sup>T)) \<^bold>\<rightarrow> (x\<^sup>T\<cdot>R1)) = X" apply simp oops
+lemma "[\<^bold>\<forall>(\<lambda>R. (R\<^sup>T\<bullet>(x\<^sup>T)) \<^bold>\<rightarrow> (x\<^sup>T\<cdot>R1))] = *" apply simp done
+lemma "\<^bold>\<forall>(\<lambda>R. (R\<^sup>T\<bullet>(x\<^sup>T)) \<^bold>\<rightarrow> (x\<^sup>T\<cdot>R1)) = X" apply simp oops
 
 
 section {* Are the priorities set correctly?*}
 
-lemma ",\<phi>, \<^bold>\<and> ,\<psi>, \<^bold>\<rightarrow> ,\<chi>, \<equiv> (,\<phi>, \<^bold>\<and> ,\<psi>,) \<^bold>\<rightarrow> ,\<chi>," apply simp done
-lemma ",\<phi>, \<^bold>\<and> ,\<psi>, \<^bold>\<rightarrow> ,\<chi>, \<equiv> ,\<phi>, \<^bold>\<and> (,\<psi>, \<^bold>\<rightarrow> ,\<chi>,)" apply simp nitpick oops
+lemma "(\<phi>\<^sup>P) \<^bold>\<and> (\<psi>\<^sup>P) \<^bold>\<rightarrow> (\<chi>\<^sup>P) \<equiv> ((\<phi>\<^sup>P) \<^bold>\<and> (\<psi>\<^sup>P)) \<^bold>\<rightarrow> (\<chi>\<^sup>P)" apply simp done
+lemma "(\<phi>\<^sup>P) \<^bold>\<and> (\<psi>\<^sup>P) \<^bold>\<rightarrow> (\<chi>\<^sup>P) \<equiv> (\<phi>\<^sup>P) \<^bold>\<and> ((\<psi>\<^sup>P) \<^bold>\<rightarrow> (\<chi>\<^sup>P))" apply simp nitpick oops
 
-lemma "(,\<phi>, \<^bold>\<and> ,\<psi>, \<^bold>\<equiv> ,\<phi>, \<^bold>\<and> ,\<psi>,) \<equiv> ((,\<phi>, \<^bold>\<and> ,\<psi>,) \<^bold>\<equiv> (,\<phi>, \<^bold>\<and> ,\<psi>,))" apply simp done
-lemma "(,\<phi>, \<^bold>\<and> ,\<psi>, \<^bold>\<equiv> ,\<phi>, \<^bold>\<and> ,\<psi>,) \<equiv> (,\<phi>, \<^bold>\<and> (,\<psi>, \<^bold>\<equiv> ,\<phi>,) \<^bold>\<and> ,\<psi>,)" apply simp nitpick oops
+lemma "((\<phi>\<^sup>P) \<^bold>\<and> (\<psi>\<^sup>P) \<^bold>\<equiv> (\<phi>\<^sup>P) \<^bold>\<and> (\<psi>\<^sup>P)) \<equiv> (((\<phi>\<^sup>P) \<^bold>\<and> (\<psi>\<^sup>P)) \<^bold>\<equiv> ((\<phi>\<^sup>P) \<^bold>\<and> (\<psi>\<^sup>P)))" apply simp done
+lemma "((\<phi>\<^sup>P) \<^bold>\<and> (\<psi>\<^sup>P) \<^bold>\<equiv> (\<phi>\<^sup>P) \<^bold>\<and> (\<psi>\<^sup>P)) \<equiv> ((\<phi>\<^sup>P) \<^bold>\<and> ((\<psi>\<^sup>P) \<^bold>\<equiv> (\<phi>\<^sup>P)) \<^bold>\<and> (\<psi>\<^sup>P))" apply simp nitpick oops
 
 
 section {* E!, O!, A! and =E *}
@@ -321,47 +395,45 @@ section {* E!, O!, A! and =E *}
 consts E::"(e\<Rightarrow>io)"
 text {* Distinguished 1-place relation constant: E! (read: ‘being concrete’ or ‘concreteness’) *}
 
-abbreviation z_ordinary::"(e\<Rightarrow>io) opt"(*<*)("O\<^sup>!")(*>*) where "O\<^sup>! \<equiv> \<lambda>\<^sup>1(\<lambda>x. \<^bold>\<diamond> <.E.\<bullet>.x.>)"
+abbreviation ordinaryObject::"(e\<Rightarrow>io) opt"(**)("O!")(**) where "O! \<equiv> \<lambda>\<^sup>1(\<lambda>x. \<^bold>\<diamond>(E\<^sup>T\<bullet>(x\<^sup>T)))"
 text {* Being ordinary is being possibly concrete. *}
 
-abbreviation z_abstract::"(e\<Rightarrow>io) opt"(*<*)("A\<^sup>!")(*>*) where "A\<^sup>! \<equiv> \<lambda>\<^sup>1(\<lambda>x. \<^bold>\<not> (\<^bold>\<diamond> <.E.\<bullet>.x.>))"
+abbreviation abstractObject::"(e\<Rightarrow>io) opt"(**)("A!")(**) where "A! \<equiv> \<lambda>\<^sup>1(\<lambda>x. \<^bold>\<not>(\<^bold>\<diamond>(E\<^sup>T\<bullet>(x\<^sup>T))))"
 text {* Being abstract is not possibly being concrete. *}
 
-abbreviation z_identity::"(e\<Rightarrow>e\<Rightarrow>io) opt"(*<*)("\<^bold>=\<^sub>e")(*>*) where "\<^bold>=\<^sub>e \<equiv> 
-  \<lambda>\<^sup>2(\<lambda>x y. ((<O\<^sup>!\<bullet>.x.> \<^bold>\<and> <O\<^sup>!\<bullet>.y.>) \<^bold>\<and> \<^bold>\<box> (\<^bold>\<forall>(\<lambda>F. <.F.\<bullet>.x.> \<^bold>\<equiv> <.F.\<bullet>.y.>))))"
+abbreviation identity::"(e\<Rightarrow>e\<Rightarrow>io) opt"(**)("\<^bold>=")(**) where "\<^bold>= \<equiv> 
+  \<lambda>\<^sup>2(\<lambda>x y. (((O!\<bullet>(x\<^sup>T)) \<^bold>\<and> (O!\<bullet>(y\<^sup>T))) \<^bold>\<and> \<^bold>\<box> (\<^bold>\<forall>(\<lambda>F. (F\<^sup>T\<bullet>(x\<^sup>T)) \<^bold>\<equiv> (F\<^sup>T\<bullet>(y\<^sup>T))))))"
 
-abbreviation z_identityE::"(e opt\<Rightarrow>e opt\<Rightarrow>io opt)"(*<*)(infixr "\<^bold>=\<^sub>E" 63)(*>*) where "x \<^bold>=\<^sub>E y \<equiv> (Exe2 \<^bold>=\<^sub>e x y)" 
-
+abbreviation identityE::"e opt\<Rightarrow>e opt\<Rightarrow>io opt"(**)(infixl "\<^bold>=\<^sub>E" 63)(**) where "x \<^bold>=\<^sub>E y \<equiv> (\<^bold>=\<bullet>x,y)"
 
 
 section {* Further test examples *}
 
-lemma "[\<^bold>\<forall>(\<lambda>x. \<^bold>\<exists>(\<lambda>R. (<.x.\<circ>.R.> \<^bold>\<rightarrow> <.x.\<circ>R1>)))] = tt" apply simp by auto
-lemma "[\<^bold>\<forall>(\<lambda>x. \<^bold>\<forall>(\<lambda>R. (<.x.\<circ>.R.> \<^bold>\<rightarrow> <.x.\<circ>R1>)))] = tt" apply simp nitpick oops
+lemma "[\<^bold>\<forall>(\<lambda>x. \<^bold>\<exists>(\<lambda>R. (x\<^sup>T\<cdot>(R\<^sup>T)) \<^bold>\<rightarrow> (x\<^sup>T\<cdot>R1)))] = \<top>" apply simp by auto
+lemma "[\<^bold>\<forall>(\<lambda>x. \<^bold>\<forall>(\<lambda>R. (x\<^sup>T\<cdot>(R\<^sup>T)) \<^bold>\<rightarrow> (x\<^sup>T\<cdot>R1)))] = \<top>" apply simp nitpick oops
 
-lemma "[a \<^bold>=\<^sub>E a] = tt" apply simp nitpick oops
+lemma "[a \<^bold>=\<^sub>E a] = \<top>" apply simp nitpick oops
 
-lemma "[<O\<^sup>!\<bullet>a> \<^bold>\<rightarrow> a \<^bold>=\<^sub>E a] = tt" apply simp done
+lemma "[(O!\<bullet>a) \<^bold>\<rightarrow> a \<^bold>=\<^sub>E a] = \<top>" apply simp done
 
-lemma "[(\<^bold>\<forall>(\<lambda>F. <.F.\<bullet>.x.> \<^bold>\<equiv> <.F.\<bullet>.x.>))] = tt" apply simp done
-lemma "[<O\<^sup>!\<bullet>a> \<^bold>\<rightarrow> <\<lambda>\<^sup>1(\<lambda>x. .x. \<^bold>=\<^sub>E a)\<bullet>a>] = tt" apply simp done
+lemma "[(\<^bold>\<forall>(\<lambda>F. (F\<^sup>T\<bullet>(x\<^sup>T)) \<^bold>\<equiv> (F\<^sup>T\<bullet>(x\<^sup>T))))] = \<top>" apply simp done
+lemma "[(O!\<bullet>a) \<^bold>\<rightarrow> ((\<lambda>\<^sup>1(\<lambda>x. (x\<^sup>T) \<^bold>=\<^sub>E a))\<bullet>a)] = \<top>" apply simp done
 
-lemma "[(\<^bold>\<exists>(\<lambda>F. <a\<circ>.F.>))] = tt" apply simp by auto
+lemma "[\<^bold>\<exists>(\<lambda>F. (a\<cdot>(F\<^sup>T)))] = \<top>" apply simp by auto
 
-lemma "[\<^bold>\<exists>(\<lambda>\<phi>. ,\<phi>,)] = tt" apply simp by auto
-lemma "[\<^bold>\<exists>(\<lambda>\<phi>. ;\<phi>;)] = tt" apply simp by auto
-
+lemma "[\<^bold>\<exists>(\<lambda>\<phi>. (\<phi>\<^sup>P))] = \<top>" apply simp by auto
+lemma "[\<^bold>\<exists>(\<lambda>\<phi>. (\<phi>\<^sup>F))] = \<top>" apply simp by auto
 
 section {* Axioms *}
 
 subsection {* Axioms for Negations and Conditionals *}
 
-lemma a21_1_PF: "[,\<phi>, \<^bold>\<rightarrow> (,\<phi>, \<^bold>\<rightarrow> ,\<phi>,)] = tt" apply simp done
-lemma a21_1_F:  "[;\<phi>; \<^bold>\<rightarrow> (;\<phi>; \<^bold>\<rightarrow> ;\<phi>;)] = tt" apply simp done
-lemma a21_2_PF: "[(,\<phi>, \<^bold>\<rightarrow> (,\<psi>, \<^bold>\<rightarrow> ,\<chi>,)) \<^bold>\<rightarrow> ((,\<phi>, \<^bold>\<rightarrow> ,\<psi>,) \<^bold>\<rightarrow> (,\<phi>, \<^bold>\<rightarrow> ,\<chi>,))] = tt" apply simp done
-lemma a21_2_F:  "[(;\<phi>; \<^bold>\<rightarrow> (;\<psi>; \<^bold>\<rightarrow> ;\<chi>;)) \<^bold>\<rightarrow> ((;\<phi>; \<^bold>\<rightarrow> ;\<psi>;) \<^bold>\<rightarrow> (;\<phi>; \<^bold>\<rightarrow> ;\<chi>;))] = tt" apply simp done
-lemma a21_3_PF: "[(\<^bold>\<not> ,\<phi>, \<^bold>\<rightarrow> \<^bold>\<not> ,\<psi>,) \<^bold>\<rightarrow> (\<^bold>\<not> ,\<phi>, \<^bold>\<rightarrow> ,\<psi>,) \<^bold>\<rightarrow> ,\<phi>,] = tt" apply simp done
-lemma a21_3_F:  "[(\<^bold>\<not> ;\<phi>; \<^bold>\<rightarrow> \<^bold>\<not> ;\<psi>;) \<^bold>\<rightarrow> (\<^bold>\<not> ;\<phi>; \<^bold>\<rightarrow> ;\<psi>;) \<^bold>\<rightarrow> ;\<phi>;] = tt" apply simp done
+lemma a21_1_P: "[(\<phi>\<^sup>P) \<^bold>\<rightarrow> ((\<phi>\<^sup>P) \<^bold>\<rightarrow> (\<phi>\<^sup>P))] = \<top>" apply simp done
+lemma a21_1_F: "[(\<phi>\<^sup>F) \<^bold>\<rightarrow> ((\<phi>\<^sup>F) \<^bold>\<rightarrow> (\<phi>\<^sup>F))] = \<top>" apply simp done
+lemma a21_2_P: "[((\<phi>\<^sup>P) \<^bold>\<rightarrow> ((\<psi>\<^sup>P) \<^bold>\<rightarrow> (\<chi>\<^sup>P))) \<^bold>\<rightarrow> (((\<phi>\<^sup>P) \<^bold>\<rightarrow> (\<psi>\<^sup>P)) \<^bold>\<rightarrow> ((\<phi>\<^sup>P) \<^bold>\<rightarrow> (\<chi>\<^sup>P)))] = \<top>" apply simp done
+lemma a21_2_F: "[((\<phi>\<^sup>F) \<^bold>\<rightarrow> ((\<psi>\<^sup>F) \<^bold>\<rightarrow> (\<chi>\<^sup>F))) \<^bold>\<rightarrow> (((\<phi>\<^sup>F) \<^bold>\<rightarrow> (\<psi>\<^sup>F)) \<^bold>\<rightarrow> ((\<phi>\<^sup>F) \<^bold>\<rightarrow> (\<chi>\<^sup>F)))] = \<top>" apply simp done
+lemma a21_3_P: "[(\<^bold>\<not>(\<phi>\<^sup>P) \<^bold>\<rightarrow> \<^bold>\<not>(\<psi>\<^sup>P)) \<^bold>\<rightarrow> ((\<^bold>\<not>(\<phi>\<^sup>P) \<^bold>\<rightarrow> (\<psi>\<^sup>P)) \<^bold>\<rightarrow> (\<phi>\<^sup>P))] = \<top>" apply simp done
+lemma a21_3_F: "[(\<^bold>\<not>(\<phi>\<^sup>F) \<^bold>\<rightarrow> \<^bold>\<not>(\<psi>\<^sup>F)) \<^bold>\<rightarrow> ((\<^bold>\<not>(\<phi>\<^sup>F) \<^bold>\<rightarrow> (\<psi>\<^sup>F)) \<^bold>\<rightarrow> (\<phi>\<^sup>F))] = \<top>" apply simp done
 
 subsection {* Axioms of Identity *}
 text {* todo *}
@@ -371,40 +443,41 @@ text {* todo *}
 
 subsection {* Axioms of Actuality *}
 
-lemma a31_1_PF: "[\<A> (\<^bold>\<not> ,\<phi>,) \<^bold>\<equiv> (\<^bold>\<not> (\<A> ,\<phi>,))] = tt" apply simp done
-lemma a31_1_F: "[\<A> (\<^bold>\<not> ;\<phi>;) \<^bold>\<equiv> (\<^bold>\<not> (\<A> ;\<phi>;))] = tt" apply simp done
-lemma a31_2_PF: "[\<A> (,\<phi>, \<^bold>\<rightarrow> ,\<psi>,) \<^bold>\<equiv> (\<A> ,\<phi>, \<^bold>\<rightarrow> \<A> ,\<psi>,)] = tt" apply simp done
-lemma a31_2_F: "[\<A> (;\<phi>; \<^bold>\<rightarrow> ;\<psi>;) \<^bold>\<equiv> (\<A> ;\<phi>; \<^bold>\<rightarrow> \<A> ;\<psi>;)] = tt" apply simp done
-lemma a31_3_PF: "[(\<A> (\<^bold>\<forall>(\<lambda>x. ,\<phi>,)) \<^bold>\<equiv> \<^bold>\<forall>(\<lambda>x. \<A> ,\<phi>,))] = tt" apply simp done
-lemma a31_3_F: "[(\<A> (\<^bold>\<forall>(\<lambda>x. ;\<phi>;)) \<^bold>\<equiv> \<^bold>\<forall>(\<lambda>x. \<A> ;\<phi>;))] = tt" apply simp done
-lemma a31_4_PF: "[\<A> ,\<phi>, \<^bold>\<equiv> \<A> (\<A> ,\<phi>,)] = tt" apply simp done
-lemma a31_4_F: "[\<A> ;\<phi>; \<^bold>\<equiv> \<A> (\<A> ;\<phi>;)] = tt" apply simp done
+lemma a31_1_P: "[\<A>(\<^bold>\<not>(\<phi>\<^sup>P)) \<^bold>\<equiv> \<^bold>\<not>(\<A>(\<phi>\<^sup>P))] = \<top>" apply simp done
+lemma a31_1_F: "[\<A>(\<^bold>\<not>(\<phi>\<^sup>F)) \<^bold>\<equiv> \<^bold>\<not>(\<A>(\<phi>\<^sup>F))] = \<top>" apply simp done
+lemma a31_2_P: "[\<A>(\<phi>\<^sup>P \<^bold>\<rightarrow> (\<psi>\<^sup>P)) \<^bold>\<equiv> (\<A>(\<phi>\<^sup>P) \<^bold>\<rightarrow> \<A>(\<psi>\<^sup>P))] = \<top>" apply simp done
+lemma a31_2_F: "[\<A>(\<phi>\<^sup>F \<^bold>\<rightarrow> (\<psi>\<^sup>F)) \<^bold>\<equiv> (\<A>(\<phi>\<^sup>F) \<^bold>\<rightarrow> \<A>(\<psi>\<^sup>F))] = \<top>" apply simp done
+lemma a31_3_P: "[\<A>(\<^bold>\<forall>(\<lambda>x. (\<phi>\<^sup>P)) \<^bold>\<equiv> \<^bold>\<forall>(\<lambda>x. \<A>(\<phi>\<^sup>P)))] = \<top>" apply simp done
+lemma a31_3_F: "[(\<A>(\<^bold>\<forall>(\<lambda>x. (\<phi>\<^sup>F))) \<^bold>\<equiv> \<^bold>\<forall>(\<lambda>x. \<A>(\<phi>\<^sup>F)))] = \<top>" apply simp done
+lemma a31_4_P: "[\<A>(\<phi>\<^sup>P) \<^bold>\<equiv> \<A>(\<A>(\<phi>\<^sup>P))] = \<top>" apply simp done
+lemma a31_4_F: "[\<A>(\<phi>\<^sup>F) \<^bold>\<equiv> \<A>(\<A>(\<phi>\<^sup>F))] = \<top>" apply simp done
 
 subsection {* Axioms of Necessity *}
 
-lemma a32_1_PF: "[\<^bold>\<box> (,\<phi>, \<^bold>\<rightarrow> ,\<phi>,) \<^bold>\<rightarrow> (\<^bold>\<box> ,\<phi>, \<^bold>\<rightarrow> \<^bold>\<box> ,\<phi>,)] = tt" apply simp done       (* K Schema *)
-lemma a32_1_F:  "[\<^bold>\<box> (;\<phi>; \<^bold>\<rightarrow> ;\<phi>;) \<^bold>\<rightarrow> (\<^bold>\<box> ;\<phi>; \<^bold>\<rightarrow> \<^bold>\<box> ;\<phi>;)] = tt" apply simp done       (* K Schema *)
-lemma a32_2_PF: "[\<^bold>\<box> ,\<phi>, \<^bold>\<rightarrow> ,\<phi>,]  = tt" apply simp done                               (* T Schema *)
-lemma a32_2_F:  "[\<^bold>\<box> ;\<phi>; \<^bold>\<rightarrow> ;\<phi>;] = tt" apply simp done                               (* T Schema *)
-lemma a32_3_PF: "[\<^bold>\<box> (\<^bold>\<diamond> ,\<phi>,) \<^bold>\<rightarrow> (\<^bold>\<diamond> ,\<phi>,)] = tt" apply simp done                       (* 5 Schema *)
-lemma a32_3_F:  "[\<^bold>\<box> (\<^bold>\<diamond> ;\<phi>;) \<^bold>\<rightarrow> (\<^bold>\<diamond> ;\<phi>;)] = tt" apply simp done                       (* 5 Schema *)
-lemma a32_4_PF: "[(\<^bold>\<forall>(\<lambda>x. \<^bold>\<box> ,\<phi>,)) \<^bold>\<rightarrow> \<^bold>\<box> (\<^bold>\<forall>(\<lambda>x. ,\<phi>,))] = tt" apply simp done           (* BF *)
-lemma a32_4_F:  "[(\<^bold>\<forall>(\<lambda>x. \<^bold>\<box> ;\<phi>;)) \<^bold>\<rightarrow> \<^bold>\<box> (\<^bold>\<forall>(\<lambda>x. ;\<phi>;))] = tt" apply simp done           (* BF *)
+lemma a32_1_P: "[(\<^bold>\<box>(\<phi>\<^sup>P \<^bold>\<rightarrow> (\<phi>\<^sup>P))) \<^bold>\<rightarrow> (\<^bold>\<box>(\<phi>\<^sup>P) \<^bold>\<rightarrow> \<^bold>\<box>(\<phi>\<^sup>P))] = \<top>" apply simp done     (* K Schema *)
+lemma a32_1_F: "[(\<^bold>\<box>(\<phi>\<^sup>F \<^bold>\<rightarrow> (\<phi>\<^sup>F))) \<^bold>\<rightarrow> (\<^bold>\<box>(\<phi>\<^sup>F) \<^bold>\<rightarrow> \<^bold>\<box>(\<phi>\<^sup>F))] = \<top>" apply simp done     (* K Schema *)
+lemma a32_2_P: "[\<^bold>\<box>(\<phi>\<^sup>P) \<^bold>\<rightarrow> (\<phi>\<^sup>P)] = \<top>" apply simp done                           (* T Schema *)
+lemma a32_2_F: "[\<^bold>\<box>(\<phi>\<^sup>F) \<^bold>\<rightarrow> (\<phi>\<^sup>F)] = \<top>" apply simp done                           (* T Schema *)
+
+lemma a32_3_P: "[\<^bold>\<box>(\<^bold>\<diamond>(\<phi>\<^sup>P)) \<^bold>\<rightarrow> \<^bold>\<diamond>(\<phi>\<^sup>P)] = \<top>" apply simp done                       (* 5 Schema *)
+lemma a32_3_F: "[\<^bold>\<box>(\<^bold>\<diamond>(\<phi>\<^sup>F)) \<^bold>\<rightarrow> \<^bold>\<diamond>(\<phi>\<^sup>F)] = \<top>" apply simp done                       (* 5 Schema *)
+lemma a32_4_P: "[\<^bold>\<forall>(\<lambda>x. \<^bold>\<box>(\<phi>\<^sup>P)) \<^bold>\<rightarrow> \<^bold>\<box>(\<^bold>\<forall>(\<lambda>x. (\<phi>\<^sup>P)))] = \<top>" apply simp done         (* BF *)
+lemma a32_4_F: "[\<^bold>\<forall>(\<lambda>x. \<^bold>\<box>(\<phi>\<^sup>F)) \<^bold>\<rightarrow> \<^bold>\<box>(\<^bold>\<forall>(\<lambda>x. (\<phi>\<^sup>F)))] = \<top>" apply simp done         (* BF *)
 
 text {* The following needs to be an axiom; it does not follow for free: it is possible that there 
 are contingently concrete individuals and it is possible that there are not: *}
 axiomatization where
-  a32_5_PF: "[\<^bold>\<diamond> (\<^bold>\<exists>(\<lambda>x. <.E.\<bullet>.x.> \<^bold>\<and> (\<^bold>\<diamond> (\<^bold>\<not> <.E.\<bullet>.x.>)))) \<^bold>\<and> \<^bold>\<diamond> (\<^bold>\<not> (\<^bold>\<exists>(\<lambda>x. <.E.\<bullet>.x.> \<^bold>\<and> (\<^bold>\<diamond> (\<^bold>\<not> <.E.\<bullet>.x.>)))))] = tt"
+  a32_5_P: "[\<^bold>\<diamond>(\<^bold>\<exists>(\<lambda>x. (E\<^sup>T\<bullet>(x\<^sup>T)) \<^bold>\<and> \<^bold>\<diamond>(\<^bold>\<not>(E\<^sup>T\<bullet>(x\<^sup>T))))) \<^bold>\<and> \<^bold>\<diamond>(\<^bold>\<not>(\<^bold>\<exists>(\<lambda>x. (E\<^sup>T\<bullet>(x\<^sup>T)) \<^bold>\<and> \<^bold>\<diamond>(\<^bold>\<not>(E\<^sup>T\<bullet>(x\<^sup>T))))))] = \<top>"
 
 subsection {* Axioms of Necessity and Actuality *}
 
-lemma a33_1_PF: "[\<A> ,\<phi>, \<^bold>\<rightarrow> \<^bold>\<box> (\<A> ,\<phi>,)] = tt" apply simp done
-lemma a33_1_F:  "[\<A> ;\<phi>; \<^bold>\<rightarrow> \<^bold>\<box> (\<A> ;\<phi>;)] = tt" apply simp done
-lemma a33_2_PF: "[\<^bold>\<box> ,\<phi>, \<^bold>\<equiv> (\<A> (\<^bold>\<box> ,\<phi>,))] = tt" apply simp done
-lemma a33_2_F:  "[\<^bold>\<box> ;\<phi>; \<^bold>\<equiv> (\<A> (\<^bold>\<box> ;\<phi>;))] = tt" apply simp done
+lemma a33_1_P: "[\<A>(\<phi>\<^sup>P) \<^bold>\<rightarrow> \<^bold>\<box>(\<A>(\<phi>\<^sup>P))] = \<top>" apply simp done
+lemma a33_1_F:  "[\<A>(\<phi>\<^sup>F) \<^bold>\<rightarrow> \<^bold>\<box>(\<A>(\<phi>\<^sup>F))] = \<top>" apply simp done
+lemma a33_2_P: "[\<^bold>\<box>(\<phi>\<^sup>P) \<^bold>\<equiv> (\<A>(\<^bold>\<box>(\<phi>\<^sup>P)))] = \<top>" apply simp done
+lemma a33_2_F:  "[\<^bold>\<box>(\<phi>\<^sup>F) \<^bold>\<equiv> (\<A>(\<^bold>\<box>(\<phi>\<^sup>F)))] = \<top>" apply simp done
 
 
-(*<*) 
+(**) 
 end
-(*>*)
+(**)
 
